theories/Prelude/Notations.v
@@ -4,6 +4,8 @@ Reserved Infix "∈" (no associativity, at level 70).
 Reserved Notation "'\['  dom '→' cod  '\]'".
 Reserved Infix "`compare`" (no associativity, at level 40).
 Reserved Infix "⊢" (no associativity, at level 70).
+Reserved Infix "⊧" (no associativity, at level 70).
+Reserved Infix "⊭" (no associativity, at level 70).
 Reserved Infix "!!" (left associativity, at level 25).
 
 Module MonadNotations.
